code/ecdsap256/Hacl.Impl.P256.Point.fsti
@@ -20,34 +20,43 @@ module SM = Hacl.Spec.P256.MontgomeryMultiplication
 inline_for_extraction noextract
 let point_seq = LSeq.lseq uint64 12
 
-let as_point_nat (p:point_seq) =
+let as_point_nat_seq (p:point_seq) =
   felem_seq_as_nat (LSeq.sub p 0 4),
   felem_seq_as_nat (LSeq.sub p 4 4),
   felem_seq_as_nat (LSeq.sub p 8 4)
 
-let point_inv (p:point_seq) =
-  let x, y, z = as_point_nat p in
+let point_inv_seq (p:point_seq) =
+  let x, y, z = as_point_nat_seq p in
   x < S.prime /\ y < S.prime /\ z < S.prime
 
 
 inline_for_extraction noextract
 let aff_point_seq = LSeq.lseq uint64 8
 
-let as_aff_point_nat (p:aff_point_seq) =
+let as_aff_point_nat_seq (p:aff_point_seq) =
   felem_seq_as_nat (LSeq.sub p 0 4),
   felem_seq_as_nat (LSeq.sub p 4 4)
 
-let aff_point_inv (p:aff_point_seq) =
-  let x, y = as_aff_point_nat p in
+let aff_point_inv_seq (p:aff_point_seq) =
+  let x, y = as_aff_point_nat_seq p in
   x < S.prime /\ y < S.prime
+
 
 
 inline_for_extraction noextract
 let point = lbuffer uint64 12ul
 
 noextract
-let point_x_as_nat (h:mem) (e:point) : GTot nat =
-  as_nat h (gsub e 0ul 4ul)
+let as_point_nat (h:mem) (p:point) =
+  as_point_nat_seq (as_seq h p)
+
+noextract
+let point_inv (h:mem) (p:point) =
+  point_inv_seq (as_seq h p)
+
+noextract
+let point_x_as_nat (h:mem) (p:point) : GTot nat =
+  as_nat h (gsub p 0ul 4ul)
 
 noextract
 let point_y_as_nat (h:mem) (e:point) : GTot nat =
@@ -81,12 +90,20 @@ inline_for_extraction noextract
 let aff_point = lbuffer uint64 8ul
 
 noextract
-let aff_point_x_as_nat (h:mem) (e:aff_point) : GTot nat =
-  as_nat h (gsub e 0ul 4ul)
+let as_aff_point_nat (h:mem) (p:aff_point) =
+  as_aff_point_nat_seq (as_seq h p)
 
 noextract
-let aff_point_y_as_nat (h:mem) (e:aff_point) : GTot nat =
-  as_nat h (gsub e 4ul 4ul)
+let aff_point_inv (h:mem) (p:aff_point) =
+  aff_point_inv_seq (as_seq h p)
+
+noextract
+let aff_point_x_as_nat (h:mem) (p:aff_point) : GTot nat =
+  as_nat h (gsub p 0ul 4ul)
+
+noextract
+let aff_point_y_as_nat (h:mem) (p:aff_point) : GTot nat =
+  as_nat h (gsub p 4ul 4ul)
 
 inline_for_extraction noextract
 let aff_getx (p:aff_point) : Stack felem
@@ -105,8 +122,8 @@ let aff_gety (p:aff_point) : Stack felem
 val make_base_point: p:point -> Stack unit
   (requires fun h -> live h p)
   (ensures fun h0 _ h1 -> modifies (loc p) h0 h1 /\
-    point_inv (as_seq h1 p) /\
-    (let (px, py, pz) = as_point_nat (as_seq h1 p) in
+    point_inv h1 p /\
+    (let (px, py, pz) = as_point_nat h1 p in
     SM.fromDomain_ px == S.g_x /\
     SM.fromDomain_ py == S.g_y /\
     SM.fromDomain_ pz == 1))
@@ -115,8 +132,8 @@ val make_base_point: p:point -> Stack unit
 val make_point_at_inf: p:point -> Stack unit
   (requires fun h -> live h p)
   (ensures fun h0 _ h1 -> modifies (loc p) h0 h1 /\
-    point_inv (as_seq h1 p) /\
-    (let (px, py, pz) = as_point_nat (as_seq h1 p) in
+    point_inv h1 p /\
+    (let (px, py, pz) = as_point_nat h1 p in
     SM.fromDomain_ px == 0 /\
     SM.fromDomain_ py == 0 /\
     SM.fromDomain_ pz == 0))
@@ -134,11 +151,11 @@ val copy_point: p:point -> res:point -> Stack unit
 val point_to_mont: p:point -> res:point -> Stack unit
   (requires fun h ->
     live h p /\ live h res /\ eq_or_disjoint p res /\
-    point_inv (as_seq h p))
+    point_inv h p)
   (ensures fun h0 _ h1 -> modifies (loc res) h0 h1 /\
-    point_inv (as_seq h1 res) /\
-   (let px, py, pz = as_point_nat (as_seq h0 p) in
-    let rx, ry, rz = as_point_nat (as_seq h1 res) in
+    point_inv h1 res /\
+   (let px, py, pz = as_point_nat h0 p in
+    let rx, ry, rz = as_point_nat h1 res in
     rx == SM.toDomain_ px /\
     ry == SM.toDomain_ py /\
     rz == SM.toDomain_ pz))
@@ -148,11 +165,11 @@ val point_to_mont: p:point -> res:point -> Stack unit
 val point_from_mont: p:point -> res:point-> Stack unit
   (requires fun h ->
     live h p /\ live h res /\ eq_or_disjoint p res /\
-    point_inv (as_seq h p))
+    point_inv h p)
   (ensures fun h0 _ h1 -> modifies (loc res) h0 h1 /\
-    point_inv (as_seq h1 res) /\
-   (let px, py, pz = as_point_nat (as_seq h0 p) in
-    let rx, ry, rz = as_point_nat (as_seq h1 res) in
+    point_inv h1 res /\
+   (let px, py, pz = as_point_nat h0 p in
+    let rx, ry, rz = as_point_nat h1 res in
     rx == SM.fromDomain_ px /\
     ry == SM.fromDomain_ py /\
     rz == SM.fromDomain_ pz))
@@ -161,19 +178,19 @@ val point_from_mont: p:point -> res:point-> Stack unit
 ///  check if a point is a point-at-infinity
 
 val is_point_at_inf: p:point -> Stack uint64
-  (requires fun h -> live h p /\ point_inv (as_seq h p))
+  (requires fun h -> live h p /\ point_inv h p)
   (ensures fun h0 r h1 -> modifies0 h0 h1 /\
     ((v r == 0 \/ v r == ones_v U64) /\
-    (if S.is_point_at_inf (SM.fromDomainPoint (as_point_nat (as_seq h0 p)))
+    (if S.is_point_at_inf (SM.fromDomainPoint (as_point_nat h0 p))
      then v r = ones_v U64 else v r = 0) /\
-    (if S.is_point_at_inf (as_point_nat (as_seq h0 p))
+    (if S.is_point_at_inf (as_point_nat h0 p)
      then v r = ones_v U64 else v r = 0)))
 
 
 val is_point_at_inf_vartime: p:point -> Stack bool
-  (requires fun h -> live h p /\ point_inv (as_seq h p))
+  (requires fun h -> live h p /\ point_inv h p)
   (ensures  fun h0 r h1 -> modifies0 h0 h1 /\
-    r == S.is_point_at_inf (as_point_nat (as_seq h0 p)))
+    r == S.is_point_at_inf (as_point_nat h0 p))
 
 
 ///  Point conversion between Jacobian and Affine coordinates representations
@@ -181,44 +198,44 @@ val is_point_at_inf_vartime: p:point -> Stack bool
 val norm_jacob_point_x: p:point -> res:felem -> Stack unit
   (requires fun h ->
     live h p /\ live h res /\ disjoint p res /\
-    point_inv (as_seq h p))
+    point_inv h p)
   (ensures fun h0 _ h1 -> modifies (loc res) h0 h1  /\
-   (let rx, _, _ = S.norm_jacob_point (SM.fromDomainPoint (as_point_nat (as_seq h0 p))) in
+   (let rx, _, _ = S.norm_jacob_point (SM.fromDomainPoint (as_point_nat h0 p)) in
     as_nat h1 res == rx))
 
 
 val norm_jacob_point: p:point -> res:point -> Stack unit
   (requires fun h ->
     live h p /\ live h res /\ eq_or_disjoint p res /\
-    point_inv (as_seq h p))
+    point_inv h p)
   (ensures fun h0 _ h1 -> modifies (loc res) h0 h1 /\
-    as_point_nat (as_seq h1 res) ==
-      S.norm_jacob_point (SM.fromDomainPoint (as_point_nat (as_seq h0 p))))
+    as_point_nat h1 res ==
+      S.norm_jacob_point (SM.fromDomainPoint (as_point_nat h0 p)))
 
 
 val to_jacob_point: p:aff_point -> res:point -> Stack unit
   (requires fun h ->
     live h p /\ live h res /\ disjoint p res /\
-    aff_point_inv (as_seq h p))
+    aff_point_inv h p)
   (ensures  fun h0 _ h1 -> modifies (loc res) h0 h1 /\
-    as_point_nat (as_seq h1 res) ==
+    as_point_nat h1 res ==
       S.to_jacob_point (aff_point_x_as_nat h0 p, aff_point_y_as_nat h0 p))
 
 
 ///  Check if a point is on the curve
 
 val is_point_on_curve_vartime: p:aff_point -> Stack bool
-  (requires fun h -> live h p /\ aff_point_inv (as_seq h p))
+  (requires fun h -> live h p /\ aff_point_inv h p)
   (ensures fun h0 r h1 -> modifies0 h0 h1 /\
-    r == S.is_point_on_curve (as_aff_point_nat (as_seq h0 p)))
+    r == S.is_point_on_curve (as_aff_point_nat h0 p))
 
 
 val aff_store_point: res:lbuffer uint8 64ul -> p:aff_point -> Stack unit
   (requires fun h ->
     live h res /\ live h p /\ disjoint res p /\
-    aff_point_inv (as_seq h p))
+    aff_point_inv h p)
   (ensures  fun h0 _ h1 -> modifies (loc res) h0 h1 /\
-    as_seq h1 res == S.aff_store_point (as_aff_point_nat (as_seq h0 p)))
+    as_seq h1 res == S.aff_store_point (as_aff_point_nat h0 p))
 
 
 val load_point_vartime: p:point -> b:lbuffer uint8 64ul -> Stack bool
@@ -226,8 +243,8 @@ val load_point_vartime: p:point -> b:lbuffer uint8 64ul -> Stack bool
     live h p /\ live h b /\ disjoint p b)
   (ensures  fun h0 res h1 -> modifies (loc p) h0 h1 /\
     (let ps = S.load_point (as_seq h0 b) in
-    (res <==> Some? ps) /\ (res ==> (point_inv (as_seq h1 p) /\
-      as_point_nat (as_seq h1 p) == Some?.v ps))))
+    (res <==> Some? ps) /\ (res ==> (point_inv h1 p /\
+      as_point_nat h1 p == Some?.v ps))))
 
 
 // TODO: mv
